

$$2, 1, 3, 5, 7, 9$$

$$1) a) 2, 5, 10, 17, 26$$

$$a_n = n^2 + 1 \quad a_1 = (1)^2 + 1 = 2 \quad a_2 = (2)^2 + 1 = 5 \quad a_3 = (3)^2 + 1 = 10$$

$$b) 0, 2, 5, 9, 14, 20$$

$$a_n = \frac{n(n+1)}{2} - 1 \quad a_1 = \frac{1(1+1)}{2} - 1 = 0 \quad a_2 = \frac{2(2+1)}{2} - 1 = 2$$

$$c) 8, 12, 17, 23, 30$$

$$a_n = \frac{(n+2)(n+3)}{2} + 2 \quad a_1 = \frac{(1+2)(1+3)}{2} + 2 = 8 \quad a_2 = \frac{(2+2)(2+3)}{2} + 2 = 12$$

$$d) 1, 5, 23, 119, 719$$

$$a_n = (n+1)! - 1 \quad a_1 = (1+1)! - 1 = 1 \quad a_2 = (2+1)! - 1 = 5$$

$$a_3 = (3+1)! - 1 = 24 - 1 = 23$$

$$3) a) a_n = \frac{1}{2}(n^2 + n) \quad a_0 = \frac{1}{2}(0^2 + 0) = 0 \quad a_1 = \frac{1}{2}(1^2 + 1) = 1 \quad a_2 = 3$$

$$a_3 = 6 \quad a_4 = 10 \quad a_n = a_{n-1} + n \quad a_2 = a_1 + 2 \quad a_1 = 0 + 1 = 1$$

$$a_0 = 0 \quad a_1 = 0 + 1 = 1 = 3$$

$$b) a_n = 2a_{n-1} - a_{n-2} \quad a_0 = 0 \quad a_1 = 1$$

$$a_2 = 2a_1 - a_0 = 2(1) - 0 = 2 \quad a_3 = 2a_2 - a_1 = 2(2) - 1 = 3$$

$$a_4 = 2a_3 - a_2 = 2(3) - 2 = 4 \quad a_5 = 2a_4 - a_3 = 2(4) - 3 = 5$$

$$a_n = n \quad a_1 = 0 \quad a_1 = 1 \quad a_2 = 2 \dots$$

$$c) a_n = n a_{n-1} \quad a_0 = 1 \quad a_1 = 1 a_0 = 1$$

$$a_2 = 2a_1 = 2 \quad a_3 = 3a_2 = 6 \quad a_4 = 4a_3 = 24$$

$$a_5 = 5a_4 = 120 \quad a_n = n! \quad a_0 = 1 \quad a_1 = 1 \quad a_2 = 2 \quad a_3 = 6$$

$$a_4 = 24 \quad a_5 = 120$$

$$5) 0, 1, 1, 2, 3, 5, 8, 13 \quad F_0 = 0$$

$$0, 0+1, 0+1+1, \dots$$

$$0, 1, 2, 0+1+1+2, 0+1+1+2+3, 0+1+1+2+3+5,$$

$$0+1+1+2+3+5+8$$

$$0, 1, 2, 4, 7, 12, 20, \dots$$

$$b) F_0 + F_1 + \dots + F_n = ?$$

$$\begin{array}{ccccccc} & 1 & 1 & 1 & 2 & 3 & 5 \\ & \swarrow & \downarrow & \swarrow & \downarrow & \swarrow & \downarrow \\ 1 & 1 & 2 & 3 & 5 & 8 & \\ 0 & 1 & 2 & 4 & 7 & 12 & 20 \end{array} \quad F_{n-2} = 1$$

2.2

$$1) 5, 9, 13, 17, 21 \dots \quad a_1 = 5$$

$$a_n = a_{n-1} + 4 \quad a_0 = 1 \quad a_1 = a_0 + 4 = 5$$

$$a_2 = a_1 + 4 = 9 \quad a_3 = a_2 + 4 = 13$$

$$b) \quad \overset{4}{5}, \overset{4}{9}, \overset{4}{13}, \overset{4}{17}, \overset{4}{21} \quad a_n = 5 + 4(n-1)$$

$$a_1 = 5 = 4 + 1 = 5 \quad a_1 = 5 + 4(1-1) = 5$$

$$a_2 = 9 = 4 + 3 + 2 = 4 + 5 \quad a_2 = 5 + 4(2-1) = 9$$

$$a_3 = 13 = 4 + 3 + 3 + 2 + 1 = 4 + 5 + 3 \quad a_3 = 5 + 4(3-1) = 13$$

$$a_4 = 17 = 4 + 4 + 3 + 3 + 3 = 4 + 5 + 8$$

$$c) \quad 2013 \text{ a term} \quad \overset{503}{4 \overline{)2012}}$$

$$a_{503} = 5 + 4(503-1) = 2013$$

$$d) \quad 5, 9, 13, 17, 21, \dots, 533 \quad \overset{133}{4 \overline{)532}}$$

$$e) \quad 5 + 9 + 13 + 17 + 21 + \dots + 533 \quad 133 \text{ terms}$$

$$\rightarrow \frac{533 + 5}{2} \cdot 133 = 35777$$

$$f) \quad b_n = ? \quad \overset{4}{5}, \overset{4}{9}, \overset{4}{13}, \overset{4}{17}, \overset{4}{21}, \dots \quad b_0 = 1$$

$$b_n = 1 + \left(\frac{4n+6}{2} \right)^n$$

$$3) \overset{2}{4} + \overset{2}{11} + \overset{2}{18} + \overset{2}{25} + \dots + 244 \quad a_0 = 1$$

$$2 = 36 \cdot 7 = 252 - 3$$

$$a_1 = 4 = 4(1) \quad a_1 = 4 + 7(n-1)$$

$$a_2 = 11 = 4 + 7$$

$$a_3 = 18 = 4 + 7 + 7$$

$$a_4 = 25 = 4 + 7 + 7 + 7$$

$$b) \frac{253 \div 36}{2} = 4554$$

$$5) \underbrace{5}_2 + \underbrace{7}_2 + \underbrace{9}_2 + \dots + 521$$

$$5 + 2(n-1) = 521$$

$$a_n = 5 + 2(n-1) \quad n = 259$$

$$S = 5 + 7 + 9 + 11 + \dots + 521 \quad 2(n-1)$$

$$+ S = 521 + 519 + 517 + 515 \dots + 5$$

$$259 \cdot 526 + 526 + 526 + 526 \dots + 526$$

$$259 \cdot \frac{259 + 526}{2} = 68117$$

2.4

$$3) a_n = a_{n-1} + 2^n \quad a_0 = 5$$

$$a_1 = a_0 + 2^1 = 7$$

$$a_2 = a_1 + 2^2 = 11$$

$$a_3 = a_2 + 2^3 = 19$$

$$a_4 = a_3 + 2^4 = 35$$

$$5, 7, 11, 19, 35$$

$$a_1 - a_0 = 2 = 2^1$$

$$a_2 - a_1 = 4 = 2^2$$

$$a_3 - a_2 = 8 = 2^3$$

$$a_4 - a_3 = 16 = 2^4$$

$$a_n - a_{n-1} = 2^n$$

$$a_n - a_0 = 2^{n+1} - 2 \quad a_n = 2^{n+1} + 3$$

$$2 = 2(1)$$

$$3 = 2 + 1$$

$$8 = 2 + 6$$

$$16 = 2 + 14$$

2.5

2) Proof: $\forall n \in \mathbb{N} \quad \sum_{k=0}^n 2^k = 2^{n+1} - 1$

1) $\overset{a_0}{2^0} + \overset{a_1}{2^1} + \overset{a_2}{2^2} + 2^3 \dots 2^n = 2^{n+1} - 1, \forall n \in \mathbb{N}$

2) $1 = 2^{0+1} - 1 = 1$

3) $2^k + 2^{k+1} = 2^{k+2} - 1 = 2^{k+1} - 1 + 2^{k+1} = 2 \cdot 2^{k+1} - 1 = 2^{k+2} - 1$

$\therefore \forall n \in \mathbb{N} \quad \sum_{k=0}^n 2^k = 2^{n+1} - 1$

□

3) Proof: $7^n - 1$ is multiple of 6, $\forall n \in \mathbb{N}$

1) $0 = 7^0 - 1 = 0$

2) $7^k - 1 = 6n \rightarrow 7^{k+1} - 1$

3) $7^{k+1} - 1 = 7^{k+1}(-7 + 6)$

$= 7(7^{k+1} - 1) + 6$

$= 7(6n) + 6$

$= 6(7n + 1) \Rightarrow n = 7n + 1 \Rightarrow 6n$

$\therefore 7^n - 1$ is multiple of 6 $\forall n \in \mathbb{N}$

□

4) Proof $1 + 3 + 5 + \dots + (2n-1) = n^2 \quad \forall n \geq 1$

1) $1 = (2(1)-1) = 1^2 = 1$

2) $2k-1 = k^2 \Rightarrow (2k-1) - (2k+1) = (k+1)^2$
 $= k^2 + (2k+1) = (k+1)^2$

$\rightarrow (k+1)^2 = k^2$

$\therefore (2n-1) = n^2 \quad \forall n \geq 1$

